checkpoint

I2SFI/CompilerPBTests.v
@@ -219,7 +219,8 @@ Definition gen_program_interface (cids : list Component.id) : G Program.interfac
                )
             ).
 
-Definition gen_value (buffers : list (Component.id*(list (Block.id * nat)))) : G value :=
+Definition gen_value (buffers : list (Component.id*(list (Block.id * nat))))
+  : G value :=
   freq [ (3%nat, (do! i <- arbitrary; returnGen (Int i)))
          ; (1%nat, (match buffers with
                   | nil => (do! i <- arbitrary; returnGen (Int i))
@@ -250,11 +251,13 @@ Definition gen_sum bsize (buffers : list (Component.id * list (Block.id * nat)))
                 returnGen (inr vals)))
        ].
 
-Definition gen_buffers (cids : list Component.id) : G (PMap.t (list (Block.id * (nat + list value)))) :=
+Definition gen_buffers (cids : list Component.id)
+  : G (PMap.t (list (Block.id * (nat + list value)))) :=
   let gen_n_buffers : G (list (Block.id * nat)) :=
       do! n <- choose (1%nat,5%nat); 
         let ids := pos_list n in
-        do! sizes <- vectorOf n (choose (1%nat, N.to_nat (SFI.SLOT_SIZE-1)%N));
+        do! sizes <- vectorOf n (choose (1%nat, N.to_nat (10)%N));
+        (* do! sizes <- vectorOf n (choose (1%nat, N.to_nat (SFI.SLOT_SIZE-1)%N)); *)
            returnGen (List.combine ids sizes) in
   do! buffers <- (vectorOf (List.length cids) gen_n_buffers);
     let comp_buffers := (List.combine cids buffers) in
@@ -273,15 +276,6 @@ Definition gen_buffers (cids : list Component.id) : G (PMap.t (list (Block.id * 
       );
     returnGen (PMapExtra.of_list (List.combine cids init_buffers)).
 
-Section CodeGeneration.
-
-  Variable pi : Program.interface.
-
-  Variable buffers : PMap.t (list (Block.id * nat)).
-
-  Variable cid : Component.id.
-
-  Variable pid : Procedure.id.
   
   Instance genOp : Gen Common.Values.binop :=
     {
@@ -307,18 +301,29 @@ Section CodeGeneration.
     }.
 
  
-  Definition genPtrImVal : G (option Intermediate.Machine.imvalue) :=
+  Definition genPtrImVal
+             (pi : Program.interface)
+              (buffers : PMap.t (list (Block.id * (nat+list value))))
+             (cid : Component.id)
+    : G (option Intermediate.Machine.imvalue) :=
     let  genPointer (id : Component.id) :=
          match PMap.find id buffers with
          | None => returnGen None
-         | Some blocks =>
-           do! b <- elements (None) (List.map Some blocks);
-             match b with
-             | None => returnGen None
-             | Some (bid,size) =>
-               do! offset <- choose (Z0,Z.of_nat size);
-                 returnGen (Some (Intermediate.Machine.IPtr ((cid,bid),offset) ))
-             end
+         | Some lst =>
+           match lst with 
+           | nil => returnGen None
+           | b::xs =>
+             do! b' <- elements b xs;
+               let '(bid,bs) := b in
+               match bs with
+               | inl size =>
+                 do! offset <- choose (Z0,Z.of_nat size);
+                   returnGen (Some (Intermediate.Machine.IPtr ((cid,bid),offset) ))
+               | inr lst =>
+                 do! offset <- choose (Z0,Z.of_nat (List.length lst));
+                   returnGen (Some (Intermediate.Machine.IPtr ((cid,bid),offset) ))
+               end
+           end
          end in    
     backtrack [
         ( 4%nat, (genPointer cid) )
@@ -332,9 +337,11 @@ Section CodeGeneration.
     do! n<-arbitrary; returnGen (Intermediate.Machine.IInt n).
   
 
-  Definition genImVal : G imvalue :=
+  Definition genImVal (pi : Program.interface)
+             (buffers : PMap.t (list (Block.id * (nat+list value))))
+             (cid : Component.id)  : G imvalue :=
     let genImValAux : G Intermediate.Machine.imvalue :=    
-        do! res <- genPtrImVal;
+        do! res <- genPtrImVal pi buffers cid;
           match res with
           | None => genIntImVal
           | Some ptr => returnGen ptr
@@ -343,8 +350,11 @@ Section CodeGeneration.
       [ (4%nat, genIntImVal)
         ; (1%nat, genImValAux) ].
 
-  Definition genIConst : G instr :=
-    do! v <- genIntImVal;
+  Definition genIConst
+             (pi : Program.interface)
+             (buffers : PMap.t (list (Block.id * (nat+list value))))
+             (cid : Component.id) : G instr :=
+    do! v <- genImVal pi buffers cid;
       do! r <- arbitrary;
       returnGen (IConst v r).
 
@@ -365,7 +375,9 @@ Section CodeGeneration.
     do! r <- arbitrary;
       returnGen (IJump r).
 
-  Definition genICall : G instr :=
+  Definition genICall (pi : Program.interface)
+             (cid : Component.id)
+             (pid : Procedure.id) : G instr :=
     match PMap.find cid pi with
     | None => returnGen INop (* This should not happen *)
     | Some comp_interface =>
@@ -408,9 +420,14 @@ Section CodeGeneration.
                                   | ILabel _ => true
                                   | _ => false
                                   end ) proc ).
-  
-  
-  Definition gen_procedure (next_label : positive) : G code :=
+
+
+  Definition gen_procedure
+             (pi : Program.interface)
+             (buffers : PMap.t (list (Block.id * (nat+list value))))
+             (cid : Component.id)
+             (pid : Procedure.id)
+             (next_label : positive) : G code :=
     let get_missing_labels proc :=
         let decl := delared_labels_in_proc proc in
         let uses :=  List.map (fun i =>
@@ -428,19 +445,19 @@ Section CodeGeneration.
                                 uses)
     in
         
-  let gen_instr  (first_label : positive)  (next_label : positive) :=
+    let gen_instr  (first_label : positive)  (next_label : positive) :=
       freq [
           (1%nat,(returnGen INop))
-          ; (4%nat, genIConst)
+          ; (4%nat, genIConst pi buffers cid)
           ; (4%nat, genILabel next_label) 
           ; (4%nat, gen2Reg IMov)
           ; (7%nat, genIBinOp)
-          ; (4%nat, gen2Reg ILoad)
+          ; (6%nat, gen2Reg ILoad)
           ; (4%nat, gen2Reg IStore)
           ; (4%nat, genIBnz first_label next_label)
-          ; (2%nat, genIJump)
-          ; (2%nat, genIJal)
-          ; (4%nat, genICall)
+          ; (8%nat, genIJump)
+          ; (8%nat, genIJal)
+          ; (6%nat, genICall pi cid pid)
           ; (4%nat, gen2Reg IAlloc)
           ; (1%nat, (returnGen IHalt))
           ; (1%nat, (returnGen IReturn))
@@ -467,8 +484,6 @@ Section CodeGeneration.
   aux [] 10%nat next_label next_label.
     
 
-End CodeGeneration.
-
 Definition gen_procs (pi : Program.interface)
            (buffers : PMap.t (list (Block.id * (nat+list value))))
   : G (PMap.t (PMap.t code)) :=
@@ -487,13 +502,14 @@ Definition gen_procs (pi : Program.interface)
        do! proc_map <- (
            foldGen
              (fun acc pid =>
-                do! proc <- gen_procedure pi cid ((max_label acc) + 1)%positive;
+                do! proc <- gen_procedure pi buffers cid pid ((max_label acc) + 1)%positive;
                 returnGen (PMap.add pid proc acc)
              ) (Component.export comp_interface) (PMap.empty code));
          (* check add labels as needed for IJal *)
          let all_decl_labels := List.fold_left
                                   (fun acc elt => (acc ++ elt)%list )
-                                  (List.map (fun p => delared_labels_in_proc (snd p)) (PMap.elements proc_map))
+                                  (List.map (fun p => delared_labels_in_proc (snd p))
+                                            (PMap.elements proc_map))
                                   (@nil positive) in
          let uses := List.fold_left
                        (fun acc elt => (acc ++ elt)%list )
@@ -507,16 +523,35 @@ Definition gen_procs (pi : Program.interface)
                                              (List.filter (fun i => match i with
                                                                  | IJal _  => true
                                                                  | _ => false
-                                                                 end ) (snd p) )) (PMap.elements proc_map))
+                                                                 end )
+                                                          (snd p) ))
+                                 (PMap.elements proc_map))
                        (@nil positive) in
          let lbls := List.nodup label_eq_dec
-                                (List.filter (fun l => Nat.eqb 0%nat (List.count_occ label_eq_dec all_decl_labels l))
-                                             uses) in
+                                (List.filter (fun l =>
+                                                Nat.eqb 0%nat
+                                                        (List.count_occ
+                                                           label_eq_dec
+                                                           all_decl_labels
+                                                           l
+                                                        )
+                                             )
+                                             uses
+                                ) in
          (* TODO do something smarter *)
          match PMap.elements proc_map with
          | nil => returnGen (PMap.add cid proc_map acc)
          | (pid,code)::_ => returnGen (PMap.add cid
-                                               (PMap.add pid ((List.map (fun l => ILabel l) lbls)++code)%list proc_map) 
+                                               (PMap.add
+                                                  pid
+                                                  (
+                                                    (
+                                                      List.map
+                                                        (fun l => ILabel l)
+                                                        lbls
+                                                    )++code
+                                                  )%list
+                                                  proc_map) 
                                                acc)
          end        
     ) (PMap.elements pi)
@@ -580,7 +615,7 @@ Conjecture correct_data_compartmentalized:
     ).
 
 
-Definition FUEL := 5000%nat.
+Definition FUEL := 500%nat.
 
 (************************************************
  * No writes outside its own memory, 
@@ -620,30 +655,63 @@ Definition show_log_entry (entry : store_log_entry) : string :=
           ++ " sfi sp: " ++ (show sfi_sp).
 
 Definition eval_store_program (p : sfi_program)
-  : (@Either (CompCert.Events.trace*MachineState.t) * store_log) :=
+  : (@Either (CompCert.Events.trace*MachineState.t*nat) * store_log ) :=
   ((CS.eval_program_with_state     
      store_log
      update_store_log
      FUEL
      p
      (RiscMachine.RegisterFile.reset_all)) nil).
-  
-Definition store_checker (log : store_log) : Checker :=
-  conjoin (List.map (fun '(pc,addr,sfi_sp) =>
-                       if (SFI.is_same_component_bool pc addr)
-                       then checker true
-                       else
-                         if (N.eqb (SFI.C_SFI addr) SFI.MONITOR_COMPONENT_ID)
-                         then
-                           whenFail ("Failed at: " ++ (show_log_entry (pc,addr,sfi_sp)) )%string
-                                    (N.eqb addr (SFI.address_of
-                                                   SFI.MONITOR_COMPONENT_ID
-                                                   (Z.to_N (2 * sfi_sp +1))
-                                                   0))
-                         else
-                           whenFail ("Failed at: " ++ (show_log_entry (pc,addr,sfi_sp)) )%string
-                                    false
-                    ) log).
+
+
+(* number of instr exec, number of internal writes, number 0f push sfi *)
+Definition store_stat := nat * nat * nat.
+
+Instance show_store_stat : Show store_stat :=
+  {|
+    show :=
+      fun ss =>
+        let '(steps, i, e) := ss in
+         "Steps: "
+           ++ (show  steps)
+           ++ " Internal: "
+           ++ (show i )
+           ++ " Push SFI: "
+           ++ (show e)
+  |}.
+             
+Definition store_stats (log : store_log) (steps : nat) : store_stat :=
+  let i := (List.length (List.filter (fun '(pc,addr,sfi_sp) =>
+                                        (SFI.is_same_component_bool pc addr)
+                                     ) log
+                        )
+           ) in
+  ((steps,i), ((List.length log) - i)%nat).
+
+Definition store_checker (log : store_log) (steps : nat) : Checker :=
+  collect
+    (store_stats log steps)
+    match log with
+    | nil => checker tt
+    | _ =>
+      conjoin (List.map (fun '(pc,addr,sfi_sp) =>
+                           if (SFI.is_same_component_bool pc addr)
+                           then checker true
+                           else
+                             if (N.eqb (SFI.C_SFI addr) SFI.MONITOR_COMPONENT_ID)
+                             then
+                               whenFail ("Failed at: "
+                                           ++ (show_log_entry (pc,addr,sfi_sp)) )%string
+                                        (N.eqb addr (SFI.address_of
+                                                       SFI.MONITOR_COMPONENT_ID
+                                                       (Z.to_N (2 * sfi_sp +1))
+                                                       0))
+                             else
+                               whenFail ("Failed at: "
+                                           ++ (show_log_entry (pc,addr,sfi_sp)) )%string
+                                        false
+                        ) log)
+    end.
 
 Definition store_correct : Checker :=
   forAll genIntermediateProgram
@@ -652,8 +720,13 @@ Definition store_correct : Checker :=
       | TargetSFI.EitherMonad.Left msg =>
         whenFail ("Compilation error: " ++ msg) false
       | TargetSFI.EitherMonad.Right p =>
-        let (res,log) := eval_store_program p in
-        store_checker log (* check the log even if the program fails *)
+        let '(res,log) := eval_store_program p in
+        match res with
+        | TargetSFI.EitherMonad.Left msg => whenFail msg (store_checker log 0%nat)
+        | TargetSFI.EitherMonad.Right (t,(mem,_,regs),steps) => 
+          (whenFail ("memory of failed program: " ++ (show_mem  mem))%string
+                    (store_checker log steps) (* check the log even if the program fails *))
+        end
       end
   ).
 
@@ -675,15 +748,19 @@ Definition update_jump_log (st : MachineState.t) (t : CompCert.Events.trace)
       if (N.eqb r RiscMachine.Register.R_RA) || (N.eqb r RiscMachine.Register.R_T)
       then
         match RiscMachine.RegisterFile.get_register r regs with
-        | Some ptr => (log ++ [TargetSFI.EitherMonad.Right (pc, RiscMachine.Memory.to_address ptr,t)])%list
+        | Some ptr => (log ++ [TargetSFI.EitherMonad.Right
+                                (pc, RiscMachine.Memory.to_address ptr,t)])%list
         | _ => log
         end
       else
-        (log ++ [TargetSFI.EitherMonad.Left ("Illegal target register: " ++ (show_N r))%string])%list
+        (log ++ [TargetSFI.EitherMonad.Left
+                   ("Illegal target register: " ++ (show_N r))%string])%list
     | RiscMachine.ISA.IJal addr => (log ++ [TargetSFI.EitherMonad.Right (pc,addr,t)])%list
     | _ => log
     end
-  | Some (RiscMachine.Data _) => (log ++ [TargetSFI.EitherMonad.Left ("Data found at address: " ++ (show pc))%string])%list
+  | Some (RiscMachine.Data _) => (log ++
+                                     [TargetSFI.EitherMonad.Left
+                                        ("Data found at address: " ++ (show pc))%string])%list
   | _ => log
   end.
             
@@ -695,36 +772,91 @@ Definition show_jump_log_entry (entry : jump_log_entry) : string :=
           ++ " trace: " ++ (show t).
 
 Definition eval_jump_program (p : sfi_program)
-  : (@Either (CompCert.Events.trace*MachineState.t) * jump_log) :=
+  : (@Either (CompCert.Events.trace*MachineState.t*nat) * jump_log) :=
   ((CS.eval_program_with_state     
      jump_log
      update_jump_log
      FUEL
      p
      (RiscMachine.RegisterFile.reset_all)) nil).
-  
-Definition jump_checker (log : jump_log) : Checker :=
-  conjoin (List.map (fun elt =>
-                       match elt with
-                       | TargetSFI.EitherMonad.Left msg => whenFail msg false
-                       | TargetSFI.EitherMonad.Right (pc,addr,t) =>
-                         if (SFI.is_same_component_bool pc addr)
-                            || (N.eqb (SFI.C_SFI addr) SFI.MONITOR_COMPONENT_ID)
-                            || (N.eqb (SFI.C_SFI pc) SFI.MONITOR_COMPONENT_ID)
-                         then
-                           match t with
-                           | nil => checker true
-                           | _ => whenFail ("Unexpectected event at log entry:" ++ (show_jump_log_entry (pc,addr,t)))
-                                          false
-                           end
-                         else
-                           match t with
-                           | _::_ => checker true
-                           | nill => whenFail ("Unexpectected empty event at log entry:" ++ (show_jump_log_entry (pc,addr,t)))
-                                             false
-                           end
-                       end
-                    ) log). (* TODO check the event too *)
+
+(* number of instr exec, number of internal jump, number of cross component jumps *)
+Definition jump_stat := nat * nat * nat.
+
+Instance show_jump_stat : Show jump_stat :=
+  {|
+    show :=
+      fun ss =>
+        let '(steps, i, e) := ss in
+         "Steps: "
+           ++ (show  steps)
+           ++ " Internal: "
+           ++ (show i )
+           ++ " Cross Component: "
+           ++ (show e)
+  |}.
+
+Definition jump_stats (log : jump_log) (steps : nat) : jump_stat :=
+  let i := (List.length
+              (List.filter
+                 (fun elt =>
+                    match elt with
+                    | TargetSFI.EitherMonad.Left msg => false
+                    | TargetSFI.EitherMonad.Right (pc,addr,t) =>
+                      (SFI.is_same_component_bool pc addr)
+                      || (N.eqb (SFI.C_SFI addr) SFI.MONITOR_COMPONENT_ID)
+                      || (N.eqb (SFI.C_SFI pc) SFI.MONITOR_COMPONENT_ID)
+                    end
+                 ) log
+              )
+           ) in
+  let e := (List.length
+              (List.filter
+                 (fun elt =>
+                    match elt with
+                    | TargetSFI.EitherMonad.Left msg => false
+                    | TargetSFI.EitherMonad.Right (pc,addr,t) =>
+                      negb (
+                          (SFI.is_same_component_bool pc addr)
+                          || (N.eqb (SFI.C_SFI addr) SFI.MONITOR_COMPONENT_ID)
+                          || (N.eqb (SFI.C_SFI pc) SFI.MONITOR_COMPONENT_ID)
+                        )
+                    end
+                 ) log
+              )
+           ) in
+  ((steps,i), e).
+
+Definition jump_checker (log : jump_log) (steps : nat) : Checker :=
+   collect
+     (jump_stats log steps)
+      match log with
+      | nil => checker tt
+      | _ =>
+        conjoin (List.map (fun elt =>
+                             match elt with
+                             | TargetSFI.EitherMonad.Left msg => whenFail msg false
+                             | TargetSFI.EitherMonad.Right (pc,addr,t) =>
+                               if (SFI.is_same_component_bool pc addr)
+                                  || (N.eqb (SFI.C_SFI addr) SFI.MONITOR_COMPONENT_ID)
+                                  || (N.eqb (SFI.C_SFI pc) SFI.MONITOR_COMPONENT_ID)
+                               then
+                                 match t with
+                                 | nil => checker true
+                                 | _ => whenFail ("Unexpectected event at log entry:"
+                                                   ++ (show_jump_log_entry (pc,addr,t)))
+                                                false
+                                 end
+                               else
+                                 match t with
+                                 | _::_ => checker true
+                                 | nill => whenFail ("Unexpectected empty event at log entry:"
+                                                      ++ (show_jump_log_entry (pc,addr,t)))
+                                                   false
+                                 end
+                             end
+                          ) log)
+      end. (* TODO check the event too *)
 
 Definition jump_correct : Checker :=
   forAll genIntermediateProgram
@@ -734,7 +866,11 @@ Definition jump_correct : Checker :=
                whenFail ("Compilation error: " ++ msg) false
              | TargetSFI.EitherMonad.Right p =>
                let (res,log) := eval_jump_program p in
-               jump_checker log (* check the log even if the program fails *)
+               match res with
+               | TargetSFI.EitherMonad.Left msg => whenFail msg (jump_checker log 0%nat)
+               | TargetSFI.EitherMonad.Right (t,(mem,_,regs),steps) => 
+                 jump_checker log steps
+               end
              end
          ).
 
@@ -751,7 +887,8 @@ Definition show_op op :=
   | Pop => "Pop"
   end.
 
-Definition cs_log_entry := RiscMachine.pc * RiscMachine.address * stack_op * RiscMachine.ISA.instr.
+Definition cs_log_entry := RiscMachine.pc * RiscMachine.address
+                           * stack_op * RiscMachine.ISA.instr.
 
 Definition cs_log := list (@Either cs_log_entry).
 
@@ -769,14 +906,17 @@ Definition update_cs_log (st : MachineState.t) (t : CompCert.Events.trace)
                        if (N.eqb r RiscMachine.Register.R_T)
                        then log
                        else
-                         (log ++ [TargetSFI.EitherMonad.Left ("Illegal target register: " ++ (show_N r))%string])%list  
+                         (log ++ [TargetSFI.EitherMonad.Left
+                                    ("Illegal target register: " ++ (show_N r))%string])%list  
                      else (* cross-component return *)
                        if (N.eqb r RiscMachine.Register.R_RA)
                        then
                          (log ++ [TargetSFI.EitherMonad.Right (pc, addr, Pop, instr)])%list
                        else
-                         (log ++ [TargetSFI.EitherMonad.Left ("Illegal target register: " ++ (show_N r))%string])%list
-        | _ => (log ++ [TargetSFI.EitherMonad.Left ("Can't find R_RA in general registers " ++ (show regs))%string])%list
+                         (log ++ [TargetSFI.EitherMonad.Left
+                                    ("Illegal target register: " ++ (show_N r))%string])%list
+        | _ => (log ++ [TargetSFI.EitherMonad.Left ("Can't find R_RA in general registers "
+                                                     ++ (show regs))%string])%list
         end
     | RiscMachine.ISA.IJal addr =>
       if SFI.is_same_component_bool pc addr
@@ -784,12 +924,15 @@ Definition update_cs_log (st : MachineState.t) (t : CompCert.Events.trace)
       else
         let '(mem',pc',regs') := st' in
         match RiscMachine.RegisterFile.get_register RiscMachine.Register.R_RA regs' with
-        | Some addr => (log ++ [TargetSFI.EitherMonad.Right (pc, RiscMachine.Memory.to_address addr,Push, instr)])%list
-        | _ => (log ++ [TargetSFI.EitherMonad.Left ("Can't find R_RA in general registers " ++ (show regs'))%string])%list
+        | Some addr => (log ++ [TargetSFI.EitherMonad.Right
+                                 (pc, RiscMachine.Memory.to_address addr,Push, instr)])%list
+        | _ => (log ++ [TargetSFI.EitherMonad.Left ("Can't find R_RA in general registers "
+                                                     ++ (show regs'))%string])%list
         end
     | _ => log
     end
-  | Some (RiscMachine.Data _) => (log ++ [TargetSFI.EitherMonad.Left ("Data found at address: " ++ (show pc))%string])%list
+  | Some (RiscMachine.Data _) => (log ++ [TargetSFI.EitherMonad.Left
+                                           ("Data found at address: " ++ (show pc))%string])%list
   | _ => log
   end.
             
@@ -802,15 +945,32 @@ Definition show_cs_log_entry (entry : cs_log_entry) : string :=
           ++ "instr " ++ (show instr). 
 
 Definition eval_cs_program (p : sfi_program)
-  : (@Either (CompCert.Events.trace*MachineState.t) * cs_log) :=
+  : (@Either (CompCert.Events.trace*MachineState.t*nat) * cs_log) :=
   ((CS.eval_program_with_state     
      cs_log
      update_cs_log
      FUEL
      p
      (RiscMachine.RegisterFile.reset_all)) nil).
+
+(* number of instr exec, number of internal jump, number of cross component jumps *)
+Definition cs_stat := nat * nat .
+
+Instance show_cs_stat : Show cs_stat :=
+  {|
+    show :=
+      fun ss =>
+        let '(steps, op) := ss in
+         "Steps: "
+           ++ (show  steps)
+           ++ " Operations no: "
+           ++ (show op )
+  |}.
+
+Definition cs_stats (log : cs_log) (steps : nat) : cs_stat :=
+  (steps, (List.length log)).
   
-Definition cs_checker (log : cs_log) : Checker :=
+Definition cs_checker (log : cs_log)  (steps : nat) : Checker :=
   let fix aux l s :=
       match l with
       | nil => checker true
@@ -839,26 +999,278 @@ Definition cs_checker (log : cs_log) : Checker :=
           end
         end
       end
-  in aux log [].
+  in
+
+  collect
+    (cs_stats log steps)
+    match steps with
+    | O => checker false
+    | _ => 
+      match log with
+      | nil => checker tt
+      | _ => aux log []
+      end
+    end.
 
 Definition cs_correct : Checker :=
   forAll genIntermediateProgram
          ( fun ip =>
              match compile_program ip with
              | TargetSFI.EitherMonad.Left msg =>
-               whenFail ("Compilation error: " ++ msg) false
+               whenFail ("Compilation error: "
+                           ++ msg
+                           ++ newline
+                           ++ (show ip) ) false
              | TargetSFI.EitherMonad.Right p =>
                let (res,log) := eval_cs_program p in
                match res with
-               | TargetSFI.EitherMonad.Left msg => whenFail msg (cs_checker log)
-               | TargetSFI.EitherMonad.Right (t,(mem,_,regs)) => 
+               | TargetSFI.EitherMonad.Left msg => whenFail msg (cs_checker log 0%nat)
+               | TargetSFI.EitherMonad.Right (t,(mem,_,regs),steps) =>
                  (whenFail ("memory of failed program: " ++ (show_mem  mem))%string
-                        (cs_checker log) (* check the log even if the program fails *))
+                        (cs_checker log steps) (* check the log even if the program fails *))
                end
              end
          ).
 
 (****************** QUICK CHECKS ***************************)
+Extract Constant Test.defNumTests => "20".
+
+(* Definition test5 *)
+(*   : @Either (sfi_program) := *)
+(*   (* : @Either (trace*MachineState.t) := *) *)
+(*   let component1_interface : Component.interface := *)
+(*       (Component.mkCompInterface [1%positive *)
+(*                                   ; 2%positive *)
+(*                                   ; 3%positive *)
+(*                                   ; 4%positive *)
+(*                                  ] [(2%positive, 3%positive)]) in *)
+(*   let component2_interface : Component.interface := *)
+(*       (Component.mkCompInterface [1%positive *)
+(*                                   ; 2%positive *)
+(*                                   ; 3%positive *)
+(*                                   ; 4%positive *)
+(*                                   ; 5%positive *)
+(*                                  ] [ *)
+(*                                    (1%positive, 3%positive) *)
+(*                                    ; (1%positive, 2%positive) *)
+(*                                    ; (3%positive, 1%positive) *)
+(*                                  ] *)
+(*       ) in *)
+(*     let component3_interface : Component.interface := *)
+(*       (Component.mkCompInterface [1%positive *)
+(*                                  ] [ *)
+(*                                    (1%positive, 3%positive) *)
+(*                                    ; (2%positive, 3%positive) *)
+(*                                    ; (2%positive, 5%positive) *)
+(*                                    ; (2%positive, 4%positive) *)
+(*                                  ] *)
+(*       ) in *)
+  
+(*     let program_interface : Program.interface := *)
+(*         PMap.add 3%positive component3_interface ( *)
+(*                    PMap.add 2%positive component2_interface ( *)
+(*                               PMap.add 1%positive *)
+(*                                        component1_interface *)
+(*                                        (PMap.empty Component.interface))) in *)
+(*   let buffers := *)
+(*       PMap.add 1%positive [(1%positive, (inl 3258%nat)) *)
+(*                          ; (2%positive,(inl 1689%nat)) *)
+(*                          ; (3%positive,(inl 1074%nat)) *)
+(*                          ; (4%positive,(inl 946%nat)) *)
+(*                          ; (5%positive,(inl 110%nat)) *)
+(*                         ] *)
+(*                (PMap.empty (list (Block.id * (nat + list value)))) in *)
+
+(*   let proc1 := *)
+(*       PMap.add *)
+(*          4%positive *)
+(*          [ IBinOp Common.Values.Eq R_AUX2 R_AUX2 R_AUX1 *)
+(*            ; IBinOp Common.Values.Leq R_AUX2 R_SP R_AUX2 *)
+(*            ; ICall 2%positive 3%positive *)
+(*            ; ILabel 10%positive *)
+(*            ; ILoad R_RA R_AUX1 *)
+(*            ; IJal 3%positive *)
+(*            ; IAlloc R_SP R_COM *)
+(*            ; IJal 19%positive *)
+(*            ; IJump R_SP *)
+(*            ; IJump R_SP *)
+(*            ; IReturn *)
+(*          ]  *)
+(*          (PMap.add *)
+(*             3%positive *)
+(*             [IJump R_AUX1 *)
+(*              ; IStore R_COM R_AUX1 *)
+(*              ; IBinOp Common.Values.Eq R_COM R_AUX1 R_AUX2 *)
+(*              ; ILabel 4%positive *)
+(*              ; IStore R_AUX2 R_SP *)
+(*              ; IBnz R_SP 4%positive *)
+(*              ; ILabel 5%positive *)
+(*              ; IBnz R_AUX1 9%positive *)
+(*              ; IMov R_AUX1 R_COM *)
+(*              ; IBinOp Common.Values.Minus R_AUX1 R_ONE R_AUX1 *)
+(*              ; ILabel 9%positive *)
+(*              ; IReturn *)
+(*             ] *)
+(*             (PMap.add *)
+(*                2%positive *)
+(*                [ILoad R_AUX1 R_COM *)
+(*                 ; IJal 20%positive *)
+(*                 ; IBinOp Common.Values.Minus R_ONE R_ONE R_COM *)
+(*                 ; ICall 2%positive 3%positive *)
+(*                 ; ILabel 2%positive *)
+(*                 ; ILabel 3%positive *)
+(*                 ; IJal 6%positive *)
+(*                 ; IJump R_AUX1 *)
+(*                 ; IBinOp Common.Values.Leq R_SP R_SP R_ONE *)
+(*                 ; ICall 2%positive 3%positive *)
+(*                 ; IReturn] *)
+(*                (PMap.add *)
+(*                   1%positive *)
+(*                   [ *)
+(*                     ILabel 17%positive *)
+(*                     ; ILabel 20%positive *)
+(*                     ; ILabel 6%positive *)
+(*                     ; ILabel 19%positive *)
+(*                     ; ILoad R_SP R_AUX1 *)
+(*                     ; IAlloc R_ONE R_COM *)
+(*                     ; IMov R_SP R_ONE *)
+(*                     ; ICall 2%positive 3%positive *)
+(*                     ; ILoad R_AUX1 R_ONE *)
+(*                     ; ILoad R_RA R_AUX1 *)
+(*                     ; ILoad R_ONE R_AUX2 *)
+(*                     ; IJal 17%positive *)
+(*                     ; IJump R_SP *)
+(*                     ; ICall 2%positive 3%positive *)
+(*                     ; IReturn *)
+(*                   ] *)
+(*                   (PMap.empty Intermediate.Machine.code)))) in *)
+(*   let proc2 := *)
+(*       PMap.add *)
+(*         5%positive *)
+(*         [ *)
+(*           ICall 3%positive 1%positive *)
+(*           ; ICall 1%positive 2%positive *)
+(*           ; ILabel 9%positive *)
+(*           ; ILoad R_ONE R_COM *)
+(*           ; IJal 20%positive *)
+(*           ; ICall 1%positive 3%positive *)
+(*           ; IJump R_AUX2 *)
+(*           ; IBinOp Common.Values.Mul R_AUX2 R_SP R_AUX2 *)
+(*           ; IBinOp Common.Values.Eq R_AUX2 R_ONE R_COM *)
+(*           ; ICall 3%positive 1%positive *)
+(*           ; IReturn *)
+(*         ] *)
+(*         ( PMap.add *)
+(*          4%positive *)
+(*          [ *)
+(*            IMov R_SP R_COM *)
+(*            ; ICall 3%positive 1%positive *)
+(*            ; IJal 4%positive *)
+(*            ; IBnz R_AUX1 8%positive *)
+(*            ; ILabel 8%positive *)
+(*            ; IJump R_AUX1 *)
+(*            ; ICall 1%positive 3%positive *)
+(*            ; IConst (IInt 4%Z) R_COM *)
+(*            ; IJal 15%positive *)
+(*            ; ILoad R_SP R_AUX2 *)
+(*            ; IReturn *)
+(*          ]  *)
+(*          (PMap.add *)
+(*             3%positive *)
+(*             [ *)
+(*               ICall 3%positive 1%positive *)
+(*               ; IJal 3%positive *)
+(*               ; ILoad R_AUX1 R_SP *)
+(*               ; IBnz R_COM 7%positive *)
+(*               ; ICall 3%positive 1%positive *)
+(*               ; ILabel 5%positive *)
+(*               ; ILoad R_ONE R_SP *)
+(*               ; ILoad R_AUX2 R_COM *)
+(*               ; IMov R_RA R_SP *)
+(*               ; IMov R_RA R_AUX2 *)
+(*               ; ILabel 7%positive *)
+(*               ; IReturn *)
+(*             ] *)
+(*             (PMap.add *)
+(*                2%positive *)
+(*                [ *)
+(*                  IStore R_SP R_COM *)
+(*                  ; IConst (IInt 3%Z) R_AUX2 *)
+(*                  ; IJal 5%positive *)
+(*                  ; IJump R_AUX2 *)
+(*                  ; IConst (IInt 1%Z) R_AUX2 *)
+(*                  ; ILoad R_AUX2 R_SP *)
+(*                  ; ICall 3%positive 1%positive *)
+(*                  ; IJal 2%positive *)
+(*                  ; ILoad R_SP R_ONE *)
+(*                  ; ICall 1%positive 2%positive *)
+(*                  ; IReturn] *)
+(*                (PMap.add *)
+(*                   1%positive *)
+(*                   [ *)
+(*                     ILabel 15%positive *)
+(*                     ; ILabel 20%positive *)
+(*                     ; ICall 1%positive 2%positive *)
+(*                     ; ICall 3%positive 1%positive *)
+(*                     ; IConst (IInt (-3)%Z) R_ONE *)
+(*                     ; ICall 3%positive 1%positive *)
+(*                     ; ILabel 2%positive *)
+(*                     ; IBnz R_COM 4%positive *)
+(*                     ; IBinOp Common.Values.Eq R_AUX1 R_ONE R_ONE *)
+(*                     ; ILabel 3%positive *)
+(*                     ; IMov R_AUX1 R_AUX2 *)
+(*                     ; INop *)
+(*                     ; ILabel 4%positive *)
+(*                     ; IReturn *)
+(*                   ] *)
+(*                   (PMap.empty Intermediate.Machine.code))))) in *)
+(*   let proc3 := PMap.add *)
+(*                   1%positive *)
+(*                   [ *)
+(*                     IJump R_SP *)
+(*                     ; IConst (IInt 3%Z) R_AUX1 *)
+(*                     ; IMov R_SP R_AUX1 *)
+(*                     ; IJump R_AUX2 *)
+(*                     ; IJump R_SP *)
+(*                     ; IAlloc R_COM R_COM *)
+(*                     ; ICall 2%positive 4%positive *)
+(*                     ; IBnz R_AUX1 4%positive *)
+(*                     ; ICall 2%positive 3%positive *)
+(*                     ; IBinOp Common.Values.Leq R_ONE R_AUX2 R_AUX2 *)
+(*                     ; ILabel 4%positive *)
+(*                     ; IReturn *)
+(*                   ] *)
+(*                   (PMap.empty Intermediate.Machine.code) in *)
+    
+(*   let procs := *)
+(*       PMap.add 1%positive proc1 *)
+(*                ( PMap.add 2%positive proc2 *)
+(*                           (PMap.add 3%positive proc3 *)
+(*                                     (PMap.empty (PMap.t Intermediate.Machine.code)))) in *)
+(*   let program : Intermediate.program := {| *)
+(*         Intermediate.prog_interface := program_interface; *)
+(*         Intermediate.prog_procedures := procs; *)
+(*         Intermediate.prog_buffers := buffers; *)
+(*         Intermediate.prog_main := (2%positive,5%positive) *)
+(*       |} in *)
+(*   compile_program program. *)
+(*   (* match compile_program program with *) *)
+(*   (* | TargetSFI.EitherMonad.Left msg => Left msg *) *)
+(*   (* | TargetSFI.EitherMonad.Right p => *) *)
+(*   (*   CS.eval_program (100%nat) p RiscMachine.RegisterFile.reset_all *) *)
+(*   (* end. *) *)
+
+(* QuickChick *)
+(*   ( let x :=  test5 in *)
+(*     match x with *)
+(*     | TargetSFI.EitherMonad.Left msg => whenFail ("Compilation failed:" *)
+(*                                                    ++ msg) *)
+(*                                                 (checker false) *)
+(*     | TargetSFI.EitherMonad.Right tp => *)
+(*       whenFail (show (mem tp) ++ "Env: " ++ (show (e tp))) (checker false) *)
+(*     end ). *)
+
+
 QuickChick store_correct.
 QuickChick jump_correct.
 QuickChick cs_correct.
